(composite-linear-transformations-section)=

```{index} Linear transformations ; composite transformations
```

# Composite linear transformations

```{prf:definition} Composite transformations
:label: composite-transformation-definition

Let $T : V \to W$ and $S: W \to X$ be two linear transformations over the vector spaces $V, W$ and $X$. The **composition** of $S$ and $T$ is the transformation $S \circ T: V \to X$ defined by

$$ (S \circ T)(\vec{u}) = S(T(\vec{u})), $$

for all vectors $\vec{u} \in V$.
```

````{prf:example}
:label: composite-transformation-example

Two linear transformations is defined as $T:(x, y, z)^\mathsf{T} \mapsto (2 x + 4 y, -x + 3 y, x + 2 y)^\mathsf{T}$ and $S:(x, y, z)^\mathsf{T} \mapsto (2x + y - z, 3x + z, y - 2z)^\mathsf{T}$, determine the composite linear transformation $S \circ T(\vec{u})$ for $\vec{u} = (x, y, z)^\mathsf{T}$.

```{dropdown} Solution
$$ \begin{align*}
    S \circ T\begin{pmatrix} x \\ y \\ z \end{pmatrix} &= 
    S \left( T\begin{pmatrix} x \\ y \\ z \end{pmatrix} \right)
    = S \begin{pmatrix} 2 x + 4 \\ - x + 3y \\ x + 2 y \end{pmatrix} \\
    &= \begin{pmatrix} 
        2(2 x + 4 y) + (-x + 3 y) - (x + 2 y) \\ 
        3(2 x + 4 y) + (x + 2 y) \\
        (-x + 3 y) - 2(x + 2 y)
    \end{pmatrix} \\
    &= \begin{pmatrix} 2 x + 9 y \\ 7 x + 14 y \\ -3 x - y \end{pmatrix}.
\end{align*} $$
```
````

## Composite transformation matrices

We have seen that a linear transformation $T: V \to W$ can be represented by a {prf:ref}`transformation matrix<transformation-matrix-definition>` so that given a vector $\vec{u} \in V$ the image is calculated using

$$ T(\vec{u}) = A \vec{u}. $$(composite-transformation-matrix-equation-1)

Consider the composition of $T$ with another linear transformation $S: W \to X$ with a transformation matrix $B$

$$ S \circ T(\vec{u}) = B \cdot T(\vec{u}) $$(composite-transformation-matrix-equation-2)

Substituting equation {eq}`composite-transformation-matrix-equation-1` into equation {eq}`composite-transformation-matrix-equation-1` gives

$$ S \circ T (\vec{u}) = B \cdot A \vec{u}. $$

```{prf:theorem} Composite transformation matrices
:label: composite-transformation-matrices-theorem

Given two linear transformations $T:V \to W$ and $S:W \to X$ with transformation matrices $A$ and $B$ respectively then the composition $S \circ T$ of the vector $\vec{u} \in V$ is[^1]

$$ S \circ T (\vec{u}) = B \cdot A \cdot \vec{u}. $$(composite-transformation-matrices-theorem-equation)
```

[^1]: This is the reason why {prf:ref}`matrix multiplication<matrix-multiplication-definition>` is defined how it is.

````{prf:example}
:label: composite-transformation-matrix-example

Calculate the transformation matrices, $A$ and $B$, for the transformations $T$ and $S$ from {prf:ref}`composite-transformation-example` and use them to calculate the transformation matrix $C$ for $S\circ T$.

```{dropdown} Solution

The transformations are $T:(x, y, z)^\mathsf{T} \mapsto (2 x + 4 y, -x + 3 y, x + 2 y)^\mathsf{T}$ and $S:(x, y, z)^\mathsf{T} \mapsto (2x + y - z, 3x + z, y - 2z)^\mathsf{T}$ which have the transformation matrices

$$ \begin{align*}
    A &= \begin{pmatrix} 2 & 4 \\ -1 & 3 \\ 1 & 2 \end{pmatrix}, &
    B &= \begin{pmatrix} 2 & 1 & - 1 \\ 3 & 0 & 1 \\ 0 & 1 & -2 \end{pmatrix}.
\end{align*} $$

Calculate the composite transformation matrix for $S \circ T$

$$ \begin{align*}
    C &= BA = \begin{pmatrix} 2 & 1 & - 1 \\ 3 & 0 & 1 \\ 0 & 1 & -2 \end{pmatrix}
    \begin{pmatrix} 2 & 4 \\ -1 & 3 \\ 1 & 2 \end{pmatrix} 
    = \begin{pmatrix} 2 & 9 \\ 7 & 14 \\ -3 & -1 \end{pmatrix}.
\end{align*} $$

Checking that $C \vec{u}$ gives the answer from {prf:ref}`composite-transformation-example`

$$ \begin{align*}
    C \cdot \begin{pmatrix} x \\ y \\ z \end{pmatrix} = 
    \begin{pmatrix} 2 & 9 \\ 7 & 14 \\ -3 & 1 \end{pmatrix}
    \begin{pmatrix} x \\ y \\ z \end{pmatrix} =
    \begin{pmatrix} 2 x + 9 y \\ 7 x + 14 y \\ -3 x + y \end{pmatrix} \quad \checkmark
\end{align*} $$
```
````
