# Shortest distance problems

```{index} Shortest distance
```

(shortest-distance-problems)=

We can take advantage of vector geometry to calculate the solutions to shortest distance problems. 

(shortest-distance-between-two-points)=

```{index} Shortest distance ; point to point
```

## Shortest distance between two points

In $\mathbb{R}^n$ the shortest distance, $d$, between two points with position vectors $\vec{p}=(p_1, p_2, \ldots, p_n)^\mathsf{T}$ and $\vec{q} = (q_1, q_2, \ldots, q_n)^\mathsf{T}$ is the length of a straight line segment connecting them. If we think about this segment as of a vector, then

$$ d = |\vec{p} - \vec{q}| = \sqrt{\displaystyle\sum_{i=1}^n (p_i-q_i)^2}. $$

Note that $|\vec{p} - \vec{q}| = |\vec{q} - \vec{p}|$.

```{index} Shortest distance ; point to line
```

## Shortest distance between a line and a point

To the shortest distance, $d$, between a line $\vec{r} = \vec{p} + t\vec{d}$ and a point with position vector $\vec{q}$ in $\mathbb{R}^n$ is the length of the vector $\vec{q} - \vec{r}$ which is perpendicular to $\vec{d}$ ({numref}`line-point-distance-figure`).

```{figure} ../_images/4_line_point_distance.svg
:name: line-point-distance-figure
:width: 450

The shortest distance of a point $\vec{q}$ from the line $\vec{r} = \vec{p} + t \vec{d}$ is the length of the vector $\vec{q} - \vec{r}$ which is perpendicular to $\vec{d}$.
```

Since $\vec{q} - \vec{r}$ is perpendicular to $\vec{d}$ then since the dot product between two perpendicular vectors is zero then

$$ \vec{d} \cdot (\vec{r} - \vec{q}) = 0, $$

Substituting the {prf:ref}`vector equation of a line<vector-equation-of-a-line-definition>`  and rearranging to make $t$ the subject gives

$$ \begin{align*}
    \vec{d} \cdot (\vec{r} - \vec{q}) &= 0 \\
    \vec{d} \cdot (\vec{p} + t \vec{d} - \vec{q}) &= 0 \\
    \vec{d} \cdot \vec{p} + t \vec{d} \cdot \vec{d} - \vec{d} \cdot \vec{q} &= 0 \\
    \therefore t &= \frac{\vec{d} \cdot \vec{q} - \vec{d} \cdot \vec{p}}{\vec{d} \cdot \vec{d}}.
\end{align*} $$

This gives the value of the parameter $t$ that can be used to calculate the position vector $\vec{r}$ and therefore the shortest distance between the point $\vec{q}$ and the line is $|\vec{q} - \vec{r}|$[^1].

[^1]: The dot product of between vector $\vec{a}$ and itself is sometimes denoted as $\vec{a}^2 = \vec{a} \cdot \vec{a}$.

```{prf:theorem} The shortest distance between a point and a line
:label: point-line-distance-theorem

The shortest distance between the point with position vector $\vec{q}$ and a line that passes through the point with position vector $\vec{p}$ in the direction $\vec{d}$ is $|\vec{q} - \vec{r}|$ where $\vec{r} = \vec{p} + t \vec{d}$ and 

$$ t = \frac{\vec{d} \cdot \vec{q} - \vec{d} \cdot \vec{p}}{\vec{d} \cdot \vec{d}}. $$(point-line-t-equation)
```

<iframe width="560" height="315" src="https://www.youtube.com/embed/4cj0TIBLM4M?si=5cknsM4ka4Xe1YHg" title="YouTube video player" frameborder="0" allow="accelerometer; autoplay; clipboard-write; encrypted-media; gyroscope; picture-in-picture; web-share" allowfullscreen></iframe>

````{prf:example}
:label: point-line-distance-example

Find the shortest distance between the point with position vector $\vec{q} = (2,2,2)^\mathsf{T}$ and the line $(t,t-2, t+1)^\mathsf{T}$.

```{dropdown} Solution

Writing the line in the form $\vec{r} = \vec{p} + t \vec{d}$ 

$$ \vec{r} = \begin{pmatrix} 0 \\ -2 \\ 1 \end{pmatrix} + t
\begin{pmatrix} 1 \\ 1 \\ 1 \end{pmatrix}, $$

so the direction vector is $\vec{d} = (1, 1, 1)$. Using equation {eq}`point-line-t-equation`

$$ \begin{align*}
    t &= \frac{\vec{d} \cdot \vec{q} - \vec{d} \cdot \vec{p}}{\vec{d} \cdot \vec{d}} \\
    &= \frac{
        \begin{pmatrix} 1 \\ 1 \\ 1 \end{pmatrix} \cdot
        \begin{pmatrix} 2 \\ 2 \\ 2 \end{pmatrix} -
        \begin{pmatrix} 1 \\ 1 \\ 1 \end{pmatrix} \cdot
        \begin{pmatrix} 0 \\ -2 \\ 1 \end{pmatrix}
    }{
        \begin{pmatrix} 1 \\ 1 \\ 1 \end{pmatrix} \cdot
        \begin{pmatrix} 1 \\ 1 \\ 1 \end{pmatrix}
    } \\
    &= \frac{6 + 1}{3} = \frac{7}{3}.
\end{align*} $$

So the point on the line which is closest to $\vec{q}$ is

$$ \begin{align*}
    \vec{r} = 
    \begin{pmatrix} 0 \\ -2 \\ 1 \end{pmatrix} + \frac{7}{3} 
    \begin{pmatrix} 1 \\ 1 \\ 1 \end{pmatrix} =
    \begin{pmatrix} 7/3 \\ 1/3 \\ 10/3 \end{pmatrix},
\end{align*} $$

and the shortest distance is $|\vec{q} - \vec{r}|$ so

$$ \begin{align*}
    \vec{q} - \vec{r} &= \begin{pmatrix} 2 \\ 2 \\ 2 \end{pmatrix} - 
    \begin{pmatrix} 7/3 \\ 1/3 \\ 10/3 \end{pmatrix} =
    \begin{pmatrix} - 1/3 \\ 5/3 \\ -4/3 \end{pmatrix}, \\
    \therefore d &= \sqrt{\left(-\frac{1}{3}\right)^2 + \left(\frac{5}{3}\right)^2 + \left( -\frac{4}{3}\right)^2} \\
    &= \sqrt{\frac{14}{3}} \approx 2.16.
\end{align*} $$
```
````

```{index} Shortest distance ; line to line
```

## Shortest distance between two lines

Given two lines $\ell_1$ and $\ell_2$ described by $\vec{r}_1 = \vec{p}_1 + t \vec{d}_1$ and $\vec{r}_2 =  \vec{p}_2 + t \vec{d}_2$ in $\mathbb{R}^n$ we have three situations to consider

- If the two lines intersect then obviously the shortest distance is obviously 0.
- If the two lines are parallel then any point on $\ell_1$ can gives the shortest distance between $\ell_1$ and $\ell_2$. Hence we simply choose a point on $\ell_2$ and apply method for {prf:ref}`finding the distance between a point and a line<point-line-distance-theorem>`.
- If the two lines are skew then the shortest distance is the distance of the chord that is perpendicular to both $\ell_1$ and $\ell_2$ ({numref}`line-line-distance-figure`).

```{figure} ../_images/4_line_line_distance.svg
:name: line-line-distance-figure
:width: 350

The shortest distance between skew lines is the distance of the chord which is perpendicular to both lines.
```

If $\vec{r}_1$ and $\vec{r}_2$ are points on the lines $\ell_1$ and $\ell_2$ respectively then the chord $\vec{r}_1 \to  \vec{r}_2$ which is perpendicular to both lines has the direction vector $\vec{n} = \vec{d}_1 \times \vec{d}_2$. If $d$ is the distance between $\vec{r}_1$ and $\vec{r}_2$ then

$$ \vec{r}_2 - \vec{r}_1 = d \left( \frac{\vec{d}_1 \times \vec{d}_2}{| \vec{d}_1 \times \vec{d}_2|} \right), $$(line-line-distance-equation-1)

Let $\hat{\vec{n}} = \dfrac{\vec{d}_1 \times \vec{d}_2}{|\vec{d}_1 \times \vec{d}_2|}$ and substituting the equations of $\vec{r}_1$ and $\vec{r}_2$ equation {eq}`line-line-distance-equation-1` gives

$$ \begin{align*}
    \vec{r}_2 - \vec{r}_1 &= d \hat{\vec{n}}\\
    (\vec{p}_2 + t_2 \vec{d}_2) - (\vec{p}_1 + t_1 \vec{d}_1) 
    &= d \hat{\vec{n}}\\
    (\vec{p}_2 + t_2 \vec{d}_2) \cdot \hat{\vec{n}} - (\vec{p}_1 + t_1 \vec{d}_1) \cdot \hat{\vec{n}} 
    &= d \hat{\vec{n}} \cdot \hat{\vec{n}} \\
    \vec{p}_2 \cdot \hat{\vec{n}} + t_2 \vec{d}_2 \cdot \hat{\vec{n}} - \vec{p}_1 \cdot \hat{\vec{n}} - t_1 \vec{d}_1 \cdot \hat{\vec{n}} 
    &= d \hat{\vec{n}} \cdot \hat{\vec{n}}.
\end{align*} $$

Since $\vec{n}$ is perpendicular to both $\ell_1$ and $\ell_2$ then $\vec{d}_1 \cdot \vec{n} = \vec{d}_2 \cdot \vec{n} = 0$ and $\hat{\vec{n}} \cdot \hat{\vec{n}} = 1$ then

$$ \vec{p}_2 \cdot \hat{\vec{n}} - \vec{p}_1 \cdot \hat{\vec{n}} = d, $$

which simplifies to

$$ d = (\vec{p}_2 - \vec{p}_1) \cdot \hat{\vec{n}}. $$

```{prf:theorem} The shortest distance between two skew lines
:label: line-line-distance-theorem

The shortest distance between two skew lines $\vec{r}_1 = \vec{p}_1 + t_1 \vec{d}_1$ and $\vec{r}_2 = \vec{p}_2 + t_2 \vec{d}_2$ is

$$ d = (\vec{p}_2 - \vec{p}_1) \cdot \hat{\vec{n}}.$$(line-line-distance-equation)

where $\hat{\vec{n}} = \dfrac{\vec{d}_1 \times \vec{d}_2}{|\vec{d}_1 \times \vec{d}_2|}$.
```

<iframe width="560" height="315" src="https://www.youtube.com/embed/4cj0TIBLM4M?si=-VjP5H3OCMDD_zOp&amp;start=304" title="YouTube video player" frameborder="0" allow="accelerometer; autoplay; clipboard-write; encrypted-media; gyroscope; picture-in-picture; web-share" allowfullscreen></iframe>

````{prf:example}
:label: line-line-distance-example

Find the shortest distance between the two skew lines $\ell_1$ and $\ell_2$ defined by $(t_1, 1 + 4t_1, 3 + 2 t_1)^\mathsf{T}$ and $(1, 1 + 2t_2, 3 + 4t_2)^\mathsf{T}$ respectively.

```{dropdown} Solution

First, we need to identify the direction vectors $\vec{d}_1$ and $\vec{d}_2$. Writing $\ell_1$ and $\ell_2$ in the form $\vec{r} = \vec{p} + t \vec{d}$ 

$$ \begin{align*}
    \vec{r}_1 &= \vec{p}_1 + t_1 \vec{d}_1 = \begin{pmatrix} 0 \\ 1 \\ 3 \end{pmatrix} + t_1
    \begin{pmatrix} 1 \\ 4 \\ 2 \end{pmatrix} , \\
    \vec{r}_2 &= \vec{p}_2 + t_2 \vec{d}_2 = \begin{pmatrix} 1 \\ 1 \\ 3 \end{pmatrix} + t_2
    \begin{pmatrix} 0 \\ 2 \\ 4 \end{pmatrix},
\end{align*} $$ 

therefore $\vec{d}_1 = (1, 4, 2)$ and $\vec{d}_2 = (0, 2, 4)$. Now we can calculate $\hat{\vec{n}}$

$$ \begin{align*}
    \vec{n} &= \vec{d}_1 \times \vec{d}_2
    = \begin{vmatrix} 
        \vec{i} & \vec{j} & \vec{k} \\
        1 & 4 & 2 \\
        0 & 2 & 4
    \end{vmatrix} = 
    \begin{pmatrix} 12 \\ -4 \\ 2 \end{pmatrix}, \\
    |\vec{n}| &= \sqrt{12^2 + (-4)^2 + 2^2} = \sqrt{164} = 2\sqrt{41}, \\
    \therefore \hat{\vec{n}} &= \frac{\vec{n}}{|\vec{n}|} 
    = \frac{1}{2\sqrt{41}}
    \begin{pmatrix} 12 \\ -4 \\ 2 \end{pmatrix} 
    = 
    \begin{pmatrix} 6\sqrt{41}/41 \\ -2\sqrt{41}/41 \\ \sqrt{41}/41 \end{pmatrix}.
\end{align*} $$

Note that since $\vec{n}$ is non-zero, $\ell_1$ and $\ell_2$ are skew lines. Using equation {eq}`line-line-distance-equation`

$$ \begin{align*}
    d &= (\vec{p}_2 - \vec{p}_1) \cdot \hat{\vec{n}} \\
    &= \left( \begin{pmatrix} 1 \\ 1 \\ 3 \end{pmatrix} -
    \begin{pmatrix} 0 \\ 1 \\ 3 \end{pmatrix} \right) \cdot 
    \begin{pmatrix} 6\sqrt{41}/41 \\ -2\sqrt{41}/41 \\ \sqrt{41}/41 \end{pmatrix} \\
    &= \begin{pmatrix} 1 \\ 0 \\ 0 \end{pmatrix} \cdot 
    \begin{pmatrix} 6\sqrt{41}/41 \\ -2\sqrt{41}/41 \\ \sqrt{41}/41 \end{pmatrix} \\
    &= \frac{6 \sqrt{41}}{41}.
\end{align*} $$
```
````
