(solving-systems-using-inverse-section)=

```{index} Solution of linear systems using the inverse matrix
```

# Solving systems of linear equations using the inverse matrix

If we have a system of linear equations of the form $A\vec{x}=\vec{b}$ where $A$ is a non-singular (invertible) square matrix then use of matrix algebra shows that

$$ \begin{align*}
    A\vec{x} &= \vec{b}\\
    A^{-1}A \vec{x} &= A^{-1}\vec{b}\\
    \vec{x} &= A^{-1}\vec{b} \qquad \text{(since $I = A^{-1}A$)}.
\end{align*} $$

```{prf:theorem} Solution of a linear system of equations using the inverse matrix
:label: solution-using-inverse-matrix-theorem

The solution to a system of linear equations $A\vec{x} = \vec{b}$ can be calculated using $\vec{x} = A^{-1}\vec{b}$.
```

Consider the system of linear equations from the [previous section](systems-of-linear-equations-chapter)

$$ \begin{pmatrix}
    2 & 1 \\
    4 & 3
\end{pmatrix}
\begin{pmatrix}
    x_1 \\ x_2
\end{pmatrix} =
\begin{pmatrix}
    4 \\ 10
\end{pmatrix}. $$

The coefficient matrix and constant vector are

$$ \begin{align*}
    A &= \begin{pmatrix}
        2 & 1 \\
        4 & 3
    \end{pmatrix}, &
    \vec{b} &= \begin{pmatrix} 4 \\ 10 \end{pmatrix},
\end{align*} $$

and the inverse of this coefficient matrix can be easily calculated using the {prf:ref}`adjoint-determinant formula<adjoint-determinant-formula-theorem>` to give

$$ A^{-1} = \begin{pmatrix}
    2 & 1 \\
    4 & 3
\end{pmatrix}^{-1}
= \frac{1}{2} \begin{pmatrix}
    3 & -1 \\
    -4 & 2
\end{pmatrix}. $$

Using $\vec{x} = A^{-1}\vec{b}$ the solution is

$$ \vec{x} = \frac{1}{2}
\begin{pmatrix}
    3 & -1 \\
    -4 & 2
\end{pmatrix}
    \begin{pmatrix} 4 \\ 10 \end{pmatrix} =
    \begin{pmatrix} 1 \\ 2 \end{pmatrix},$$

so $x_1 = 1$ and $x_2 = 2$ (which we saw when we used [algebra to solve this system](solving-systems-of-linear-equations-using-algebra-section)). We can check whether this is the correct solution by substituting $\vec{x}$ into $A\vec{x} = \vec{b}$

$$A \vec{x} = \begin{pmatrix} 2 & 1 \\ 4 & 3 \end{pmatrix}
    \begin{pmatrix} 1 \\ 2 \end{pmatrix} =
    \begin{pmatrix} 4 \\ 10 \end{pmatrix} = \vec{b}.$$




<iframe width="560" height="315" src="https://www.youtube.com/embed/sMFYn2-RB7E?si=Fl_s8L4zYsMxfuuU" title="YouTube video player" frameborder="0" allow="accelerometer; autoplay; clipboard-write; encrypted-media; gyroscope; picture-in-picture; web-share" allowfullscreen></iframe>

````{prf:example}
:label: solution-by-inverse-example

Solve the following systems of linear equations using the inverse of the coefficient matrix:

(i) &emsp; $\begin{array}{rl}
        x_1 - 2x_2  \!\!\!\! &= 11, \\
        2x_1 + 4x_2  \!\!\!\! &= -18.
    \end{array}$

```{dropdown} Solution (click to show)
Here $A = \begin{pmatrix} 1 & -2 \\ 2 & 4 \end{pmatrix}$ and $\vec{b} = \begin{pmatrix} 11 \\ -18 \end{pmatrix}$. Calculating $A^{-1}$

$$ \begin{align*}
    \det\begin{pmatrix} 1 & -2 \\ 2 & 4 \end{pmatrix} &= 8, \\
    \operatorname{adj}\begin{pmatrix} 1 & -2 \\ 2 & 4 \end{pmatrix} &= 
    \begin{pmatrix} 4 & -2 \\ 2 & 1 \end{pmatrix}^\mathsf{T} = 
    \begin{pmatrix} 4 & 2 \\ -2 & 1 \end{pmatrix},\\
    \therefore A^{-1} &= \frac{1}{8} \begin{pmatrix} 4 & 2 \\ -2 & 1 \end{pmatrix}.
\end{align*} $$

So the solution is

$$ \begin{align*}
    \vec{x} &= \frac{1}{8} \begin{pmatrix} 4 & 2 \\ -2 & 1 \end{pmatrix}
    \begin{pmatrix} 11 \\ -18 \end{pmatrix} = 
    \frac{1}{8} \begin{pmatrix} 8 \\ -40 \end{pmatrix} = 
    \begin{pmatrix} 1 \\ -5 \end{pmatrix}. 
\end{align*} $$

Checking the solution

$$A\vec{x} = \begin{pmatrix} 1 & -2 \\ 2 & 4 \end{pmatrix} \begin{pmatrix} 1 \\ -5 \end{pmatrix} = \begin{pmatrix}  11 \\  -18    \end{pmatrix}  = \vec{b} \qquad \checkmark$$
```

(ii) &emsp; $\begin{array}{rl}
        x_1 - 2x_2 + 3x_3 \!\!\!\! &= -7, \\
        2x_2 - 4x_3  \!\!\!\! &= 8, \\
        3x_1 + x_2 - 4x_3  \!\!\!\! &= 7.
    \end{array}$

```{dropdown} Solution (click to show)
Here $A = \begin{pmatrix} 1 & -2 & 3 \\ 0 & 2 & -4 \\ 3 & 1 & -4 \end{pmatrix}$ and $\vec{b} = \begin{pmatrix}-7 \\ 8 \\ 7 \end{pmatrix}$. Calculating $A^{-1}$

$$ \begin{align*}
    \det \begin{pmatrix} 1 & -2 & 3 \\ 0 & 2 & -4 \\ 3 & 1 & -4 \end{pmatrix} &= 
    \begin{vmatrix} 2 & -4 \\ 1 & -4 \end{vmatrix} + 
    3 \begin{vmatrix} -2 & 3 \\ 2 & -4 \end{vmatrix} = -4 + 3(2) = 2, \\
    \operatorname{adj} \begin{pmatrix} 1 & -2 & 3 \\ 0 & 2 & -4 \\ 3 & 1 & -4 \end{pmatrix}
    &= \begin{pmatrix} -4 & -12 & -6 \\ -5 & -13 & -7 \\ 2 & 4 & 2 \end{pmatrix}^\mathsf{T} 
    = \begin{pmatrix} -4 & -5 & 2 \\ -12 & -13 & 4 \\ -6 & -7 & 2 \end{pmatrix}, \\
    \therefore A^{-1} &= \frac{1}{2}
    \begin{pmatrix}
        -4 & -5 & 2 \\
        -12 & -13 & 4 \\
        -6 & -7 & 2
    \end{pmatrix}.
\end{align*} $$

So the solution is

$$ \begin{align*}
    \vec{x} &= \frac{1}{2}
    \begin{pmatrix}
        -4 & -5 & 2 \\
        -12 & -13 & 4 \\
        -6 & -7 & 2
    \end{pmatrix}
    \begin{pmatrix}-7 \\ 8 \\ 7 \end{pmatrix}
    = \frac{1}{2} \begin{pmatrix} 2 \\ 8 \\ 0 \end{pmatrix}
    = \begin{pmatrix} 1 \\4 \\ 0 \end{pmatrix}.
\end{align*} $$

Checking the solution

$$A \vec{x} = \begin{pmatrix} 1 & -2 &  3 \\ 0 & 2 & -4 \\ 3 & 1 & -4 \end{pmatrix} \begin{pmatrix} 1 \\ 4 \\ 0 \end{pmatrix} = \begin{pmatrix} -7 \\ 8 \\ 7 \end{pmatrix} = \vec{b} \qquad \checkmark$$
```
````
