(composite-linear-transformations-section)=

:::{index} Linear transformations ; composite transformations
:::

# Composite linear transformations

:::{prf:definition} Composite transformations
:label: composite-transformation-definition

Let $S : V \to W$ and $T: W \to X$ be two linear transformations over the vector spaces $V, W$ and $X$. The **composition** of $S$ and $T$ is the transformation $S \circ T: V \to X$ defined by

$$ (S \circ T)(\mathbf{u}) = S(T(\mathbf{u})), $$

for all vectors $\mathbf{u} \in V$.
:::

::::{prf:example}
:label: composite-transformation-example

Two linear transformations is defined as $T:(x, y, z) \mapsto (2 x + 4 y, -x + 3 y, x + 2 y)$ and $S:(x, y) \mapsto (2x + y - z, 3x + z, y - 2z)$, determine the composite linear transformation $S \circ T(\mathbf{u})$ for $\mathbf{u} = (x, y, z)$.

:::{dropdown} Solution (click to reveal)
\begin{align*}
    S \circ T\begin{pmatrix} x \\ y \\ z \end{pmatrix} &= 
    S \left( T\begin{pmatrix} x \\ y \\ z \end{pmatrix} \right)
    = S \begin{pmatrix} 2 x + 4 \\ - x + 3y \\ x + 2 y \end{pmatrix} \\
    &= \begin{pmatrix} 
        2(2 x + 4 y) + (-x + 3 y) - (x + 2 y) \\ 
        3(2 x + 4 y) + (x + 2 y) \\
        (-x + 3 y) - 2(x + 2 y)
    \end{pmatrix} \\
    &= \begin{pmatrix} 2 x + 9 y \\ 7 x + 14 y \\ -3 x - y \end{pmatrix}.
\end{align*}
:::
::::

## Composite transformation matrices

We have seen that a linear transformation $T: V \to W$ can be represented by a {prf:ref}`transformation matrix<transformation-matrix-definition>` so that given a vector $\mathbf{u} \in V$ the image is calculated using

$$ T(\mathbf{u}) = A \mathbf{u}. $$(composite-transformation-matrix-equation-1)

Consider the composition of $T$ with another linear transformation $S: W \to X$ with a transformation matrix $B$

$$ S \circ T(\mathbf{u}) = B \cdot T(\mathbf{u}) $$(composite-transformation-matrix-equation-2)

Substituting equation {eq}`composite-transformation-matrix-equation-1` into equation {eq}`composite-transformation-matrix-equation-1` gives

$$ S \circ T (\mathbf{u}) = B \cdot A \mathbf{u}. $$

:::{prf:theorem} Composite transformation matrices
:label: composite-transformation-matrices-theorem

Given two linear transformations $T:V \to W$ and $S:W \to X$ with transformation matrices $A$ and $B$ respectively then the composition $S \circ T$ of the vector $\mathbf{u} \in V$ is 

$$ S \circ T (\mathbf{u}) = B \cdot A \mathbf{u}. $$(composite-transformation-matrices-theorem-equation)
:::

::::{prf:example}
:label: composite-transformation-matrix-example

Calculate the transformation matrices, $A$ and $B$, for the transformations $T$ and $S$ from {prf:ref}`composite-transformation-example` and use them to calculate the transformation matrix $C$ for $S\circ T$. 

:::{dropdown} Solution (click to reveal)
\begin{align*}
    A &= \begin{pmatrix} 2 & 4 \\ -1 & 3 \\ 1 & 2 \end{pmatrix}, \\
    B &= \begin{pmatrix} 2 & 1 & - 1 \\ 3 & 0 & 1 \\ 0 & 1 & -2 \end{pmatrix}, \\ 
    \therefore C &= BA = \begin{pmatrix} 2 & 1 & - 1 \\ 3 & 0 & 1 \\ 0 & 1 & -2 \end{pmatrix}
    \begin{pmatrix} 2 & 4 \\ -1 & 3 \\ 1 & 2 \end{pmatrix} \\
    &= \begin{pmatrix} 2 & 9 \\ 7 & 14 \\ -3 & 1 \end{pmatrix}.
\end{align*}

Checking that $C \mathbf{u}$ gives the answer from {prf:ref}`composite-transformation-example`

\begin{align*}
    C \cdot \begin{pmatrix} x \\ y \\ z \end{pmatrix} = 
    \begin{pmatrix} 2 & 9 \\ 7 & 14 \\ -3 & 1 \end{pmatrix}
    \begin{pmatrix} x \\ y \\ z \end{pmatrix} =
    \begin{pmatrix} 2 x + 9 y \\ 7 x + 14 y \\ -3 x + y \end{pmatrix} \quad \checkmark
\end{align*}
:::
::::
